Trying to make dpairs work with Theo's suggestions

rupicola/stlc_v2/Compiler.fst
@@ -9,43 +9,122 @@ open STLC
 open TypRel
 open ExpRel
 
-class compile_typ (g:env) (s:fs_env g -> Type) = {
+type fs_otyp (g:env) =
+  fs_env g -> Type
+
+class compile_otyp (g:env) (s:fs_otyp g) = {
   [@@@no_method] r : (fs_s:fs_env g -> rtyp (s fs_s));
 }
+unfold let compile_typ (s:Type) = compile_otyp empty (fun _ -> s)
 
-instance compile_typ_unit : compile_typ unit = { r = RUnit }
-instance compile_typ_bool : compile_typ bool = { r = RBool }
-instance compile_typ_arrow (s1:Type) (s2:Type) {| c1:compile_typ s1 |} {| c2:compile_typ s2 |} : compile_typ (s1 -> s2) = { r = RArr c1.r c2.r }
-instance compile_typ_pair (s1:Type) (s2:Type) {| c1:compile_typ s1 |} {| c2:compile_typ s2 |} : compile_typ (s1 & s2) = { r = RPair c1.r c2.r }
+let pack #g #ot (c:compile_otyp g ot) : otyp g = fun s -> (| ot s, c.r s |)
 
-instance compile_typ_dpair (s1:Type) (s2:s1 -> Type) {| c1:compile_typ s1 |} {| c2:(x:s1 -> compile_typ (s2 x)) |} : compile_typ (x:s1 & s2 x) = {
-  r = RDPair c1.r s2 (fun x -> (| (c2 x).t, (c2 x).r |)) }
+instance compile_typ_unit g : compile_otyp g (fun _ -> unit) = { r = fun _ -> RUnit }
+instance compile_typ_bool g : compile_otyp g (fun _ -> bool) = { r = fun _ -> RBool }
+instance compile_typ_arrow g (s1:fs_otyp g) (s2:fs_otyp g) {| c1:compile_otyp g s1 |} {| c2:compile_otyp g s2 |}
+  : compile_otyp g (fun s -> (s1 s) -> (s2 s)) = { r = fun s -> RArr (c1.r s) (c2.r s) }
 
-let pack #s (c:compile_typ s) : typsr = (| s, c.r |)
+instance compile_typ_pair g (s1:fs_otyp g) (s2:fs_otyp g) {| c1:compile_otyp g s1 |} {| c2:compile_otyp g s2 |}
+  : compile_otyp g (fun s -> (s1 s) & (s2 s)) = { r = fun s -> RPair (c1.r s) (c2.r s) }
 
 // Some tests
 let test0 : compile_typ (unit) = solve
-let _ = assert (test0.r == RUnit)
+let _ = assert (test0.r fs_empty == RUnit)
 let test1 : compile_typ (bool -> unit) = solve
-let _ = assert (test1.r == (RArr RBool RUnit))
+let _ = assert (test1.r fs_empty == (RArr RBool RUnit))
+
+instance compile_typ_dpair g (s1:fs_otyp g) (s2:(s:fs_env g -> s1 s -> fs_otyp g)) {| c1:compile_otyp g s1 |} {| c2:(s:fs_env g -> x:s1 s -> compile_otyp g (s2 s x)) |}
+  : compile_otyp g (fun s -> x:(s1 s) & (s2 s x s)) = {
+    r = fun s -> RDPair (c1.r s) (fun x -> s2 s x s) (fun x -> (c2 s x).r s)
+  }
+
+instance compile_typ_dpair' g
+  (s1:fs_otyp g) {| c1:compile_otyp g s1 |}
+  (s2:(s:fs_env g -> fs_otyp (extend (pack c1 s) g))) {| c2:(s:fs_env g -> compile_otyp (extend (pack c1 s) g) (s2 s)) |}
+  : compile_otyp g (fun s -> x:(s1 s) & (s2 s (fs_extend s x))) = {
+    r = fun s -> RDPair (c1.r s) (fun x -> s2 s (fs_extend s x)) (fun x -> (c2 s).r (fs_extend s x))
+  }
+
+(** To extend g with s1, I need an evaluation environment????
+
+I think we need a different notion of typing environment and evaluation environment to make this work.
+
+val env
+val extend : g:env -> (fs_otyp g) -> env
+
+
+instance compile_typ_dpair''
+  g
+  (s1:fs_otyp g) {| c1:compile_otyp g s1 |}
+  (s2:(fs_otyp (extend s g))) {| c2:compile_otyp (extend s g) s |}
+  : compile_otyp g (fun s -> x:(s1 s) & (s2 (fs_extend s x))) = {
+    r = fun s -> RDPair (c1.r s) (fun x -> s2 (fs_extend s x)) (fun x -> c2.r (fs_extend s x))
+  }
+
+type fs_oexp #g (a:fs_otyp g) =
+  s:fs_env g -> a s
+
+class compile_exp (#g:env) (a:fs_otyp g) {| ca: compile_otyp g a |} (fs_e:fs_oexp a) = {
+  e : (e:exp{fv_in_env g e}); (** expression is closed by g *)
+}
+
+instance compile_exp_dpair
+  g
+  (a:fs_otyp g)                            {| ca: compile_otyp g a |}
+  (b:fs_otyp (extend a g))                 {| c2: compile_otyp (extend a g) b |}
+  (l:fs_oexp a)                            {| cl: compile_exp a #ca l |}
+  (r:fs_oexp b)                            {| cr: compile_exp b #cb r |} (** this cannot be general because we only have `l fs` **)
+  : compile_exp g (fun s -> (x:a s & b (extend s x))) (fun fs_s -> (| l s, r (extend s (l s)) |)) = {
+  e = EPair cl.e cr.e
+**)
+
 
 let test_typ_dpair : compile_typ (b:bool & (if b then unit else bool)) =
   compile_typ_dpair
-    bool
-    (fun x -> if x then unit else bool)
+    empty
+    (fun _ -> bool)
+    (fun _ x _ -> if x then unit else bool)
     #solve
-    #(fun x -> if x then compile_typ_unit else compile_typ_bool)
+    #(fun _ x -> if x then compile_typ_unit empty else compile_typ_bool empty)
+
+[@expect_failure] // TODO
+let test_typ_dpair' : compile_typ (b:bool & (if b then unit else bool)) =
+  compile_typ_dpair'
+    empty
+    (fun _ -> bool)
+    (fun _ s -> if get_v s 0 then unit else bool)
+    #solve
+    #(fun _ -> ({ r = fun s -> if get_v s 0 then RUnit else RBool }))
 
 let test2 : compile_typ ((unit -> bool) -> (bool -> unit)) = solve
-let _ = assert (test2.r == RArr (RArr RUnit RBool) (RArr RBool RUnit))
+
+let _ = assert (test2.r fs_empty == RArr (RArr RUnit RBool) (RArr RBool RUnit))
 
 (** Compiling expressions **)
-class compile_exp (g:env) (#a:fs_env g -> Type0) {| ca: compile_typ g a |} (fs_e:(s:fs_env g -> a s)) = {
+class compile_exp (g:env) (#a:fs_otyp g) {| ca: compile_otyp g a |} (fs_e:fs_oexp (pack ca)) = {
   [@@@no_method] e : (e:exp{fv_in_env g e}); (** expression is closed by g *)
 
   (** The following two lemmas are independent one of the other (we don't use one to prove the other). **)
  // [@@@no_method] typing_proof : unit -> Lemma (sem_typing g e ca.t);
-  [@@@no_method] equiv_proof : unit -> Lemma (fs_e `equiv (pack ca)` e);
+  [@@@no_method] equiv_proof : unit -> Lemma (requires False) (ensures (fs_e `equiv (pack ca)` e));
+}
+
+instance compile_exp_dpair
+  g
+  (a:fs_otyp g)                           {| ca: compile_typ a |}
+  (b:(s:fs_env g -> a s -> fs_otyp g))      {| c2:(s:fs_env g -> x:a s -> compile_otyp g (b s x)) |}
+  (l:fs_env empty -> a)                    {| cl: compile_exp #_ #ca empty l |}
+  (r:(fs:fs_env empty -> b (l fs)))        {| cr: compile_closed #_ #(cb (l fs)) (r fs) |} (** this cannot be general because we only have `l fs` **)
+  : compile_exp #(x:a & b x) empty (fun fs_s -> (| l fs_s, r fs_s |)) = {
+  e = begin
+    EPair cl.e (cr fs_empty).e (** having the F* evaluation environment here, `fs`,
+                                   is not possible because of the lambda instance where
+                                   we would have to pass an extended environment to get the body,
+                                   which we cannot do because we do not have any F* argument there **)
+  end;
+  equiv_proof = (fun () ->
+    admit ()
+  );
 }
 
 (** Just a helper typeclass **)
@@ -359,7 +438,7 @@ instance compile_exp_dpair
   (a:Type)                                {| ca: compile_typ a |}
   (b:a -> Type)                            {| cb: (x:a -> compile_typ (b x) g) |}
   (l:fs_env empty -> a)                    {| cl: compile_exp #_ #ca empty l |}
-  (r:(fs:fs_env empty -> b (l fs)))        {| cr: compile_closed #_ #(cb (l fs)) (r fs)) |} (** this cannot be general because we only have `l fs` **)
+  (r:(fs:fs_env empty -> b (l fs)))        {| cr: compile_closed #_ #(cb (l fs)) (r fs) |} (** this cannot be general because we only have `l fs` **)
   : compile_exp #(x:a & b x) empty (fun fs_s -> (| l fs_s, r fs_s |)) = {
   e = begin
     EPair cl.e (cr fs_empty).e (** having the F* evaluation environment here, `fs`,
